proofs/fstar/extraction/Sandwich.Tunnel.Tls.fsti
@@ -19,6 +19,23 @@ type t_TlsVersion =
 val t_TlsVersion_cast_to_repr (x: t_TlsVersion)
     : Prims.Pure isize Prims.l_True (fun _ -> Prims.l_True)
 
+/// A set of security requirements that can be updated with new requirements
+/// described in a given verifier `V`.
+/// A sanitizer check for security requirements described in a given verifier
+/// `V`.
+class t_VerifierSanitizer (#v_Self: Type0) (#v_V: Type0) = {
+  f_run_sanitizer_checks_pre:v_Self -> v_V -> bool;
+  f_run_sanitizer_checks_post:
+      v_Self ->
+      v_V ->
+      Core.Result.t_Result Prims.unit Sandwich.Error.t_Error
+    -> bool;
+  f_run_sanitizer_checks:x0: v_Self -> x1: v_V
+    -> Prims.Pure (Core.Result.t_Result Prims.unit Sandwich.Error.t_Error)
+        (f_run_sanitizer_checks_pre x0 x1)
+        (fun result -> f_run_sanitizer_checks_post x0 x1 result)
+}
+
 /// Verify mode.
 type t_VerifyMode =
   | VerifyMode_None : t_VerifyMode
@@ -67,8 +84,8 @@ type t_TunnelSecurityRequirements = { f_allow_expired_certificate:bool }
 
 /// Instantiates a [`TunnelSecurityRequirements`] from a [`pb_api::X509Verifier`].
 [@@ FStar.Tactics.Typeclasses.tcinstance]
-let impl: Core.Convert.t_From t_TunnelSecurityRequirements
-  Sandwich_api_proto.Verifiers.t_X509Verifier =
+let impl: Core.Convert.t_From #t_TunnelSecurityRequirements
+  #Sandwich_api_proto.Verifiers.t_X509Verifier =
   {
     f_from_pre = (fun (x509_verifier: Sandwich_api_proto.Verifiers.t_X509Verifier) -> true);
     f_from_post
@@ -96,7 +113,7 @@ val impl__TunnelSecurityRequirements__new: Prims.unit
 
 /// Implements [`Default`] for [`TunnelSecurityRequirements`].
 [@@ FStar.Tactics.Typeclasses.tcinstance]
-let impl_1: Core.Default.t_Default t_TunnelSecurityRequirements =
+let impl_1: Core.Default.t_Default #t_TunnelSecurityRequirements =
   {
     f_default_pre = (fun (_: Prims.unit) -> true);
     f_default_post = (fun (_: Prims.unit) (out: t_TunnelSecurityRequirements) -> true);
@@ -115,28 +132,11 @@ val impl__TunnelSecurityRequirements__openssl3_assess_x509_store_error
       (error: i32)
     : Prims.Pure bool Prims.l_True (fun _ -> Prims.l_True)
 
-/// A set of security requirements that can be updated with new requirements
-/// described in a given verifier `V`.
-/// A sanitizer check for security requirements described in a given verifier
-/// `V`.
-class t_VerifierSanitizer (v_Self: Type0) (v_V: Type0) = {
-  f_run_sanitizer_checks_pre:v_Self -> v_V -> bool;
-  f_run_sanitizer_checks_post:
-      v_Self ->
-      v_V ->
-      Core.Result.t_Result Prims.unit Sandwich.Error.t_Error
-    -> bool;
-  f_run_sanitizer_checks:x0: v_Self -> x1: v_V
-    -> Prims.Pure (Core.Result.t_Result Prims.unit Sandwich.Error.t_Error)
-        (f_run_sanitizer_checks_pre x0 x1)
-        (fun result -> f_run_sanitizer_checks_post x0 x1 result)
-}
-
 /// Implements [`VerifierSanitizer`] for [`TunnelSecurityRequirements`]
 /// with the [`pb_api::SANVerifier`] verifier.
 [@@ FStar.Tactics.Typeclasses.tcinstance]
-let impl_3: t_VerifierSanitizer t_TunnelSecurityRequirements
-  Sandwich_api_proto.Verifiers.t_SANVerifier =
+let impl_3: t_VerifierSanitizer #t_TunnelSecurityRequirements
+  #Sandwich_api_proto.Verifiers.t_SANVerifier =
   {
     f_run_sanitizer_checks_pre
     =
@@ -165,7 +165,7 @@ let impl_3: t_VerifierSanitizer t_TunnelSecurityRequirements
                 #Alloc.Alloc.t_Global
                 verifier.Sandwich_api_proto.Verifiers.f_alt_names
             then
-              let! hoist3:Rust_primitives.Hax.t_Never =
+              let! hoist4:Rust_primitives.Hax.t_Never =
                 Core.Ops.Control_flow.ControlFlow_Break
                 (Core.Result.Result_Err
                   (Core.Convert.f_into #(Sandwich_proto.Errors.t_TunnelError & string)
@@ -183,7 +183,7 @@ let impl_3: t_VerifierSanitizer t_TunnelSecurityRequirements
                   (Core.Result.t_Result Prims.unit Sandwich.Error.t_Error)
                   Rust_primitives.Hax.t_Never
               in
-              Core.Ops.Control_flow.ControlFlow_Continue (Rust_primitives.Hax.never_to_any hoist3)
+              Core.Ops.Control_flow.ControlFlow_Continue (Rust_primitives.Hax.never_to_any hoist4)
               <:
               Core.Ops.Control_flow.t_ControlFlow
                 (Core.Result.t_Result Prims.unit Sandwich.Error.t_Error) Prims.unit
@@ -219,7 +219,7 @@ let impl_3: t_VerifierSanitizer t_TunnelSecurityRequirements
                 (fun temp_0_ temp_1_ ->
                     let has_email, has_ip:(bool & bool) = temp_0_ in
                     let i, san:(usize & Sandwich_api_proto.Verifiers.t_SANMatcher) = temp_1_ in
-                    let (has_email, has_ip), hoist4:((bool & bool) &
+                    let (has_email, has_ip), hoist5:((bool & bool) &
                       Core.Result.t_Result Prims.unit Sandwich.Error.Code.t_ErrorCode) =
                       match
                         Core.Option.impl__as_ref #Sandwich_api_proto.Verifiers.Sanmatcher.t_San
@@ -378,7 +378,7 @@ let impl_3: t_VerifierSanitizer t_TunnelSecurityRequirements
                         ((bool & bool) &
                           Core.Result.t_Result Prims.unit Sandwich.Error.Code.t_ErrorCode)
                     in
-                    match hoist4 with
+                    match hoist5 with
                     | Core.Result.Result_Ok ok ->
                       Core.Ops.Control_flow.ControlFlow_Continue
                       (has_email, has_ip <: (bool & bool))
@@ -413,8 +413,8 @@ let impl_3: t_VerifierSanitizer t_TunnelSecurityRequirements
 /// Implements [`VerifierSanitizer`] for [`TunnelSecurityRequirements`]
 /// with the [`pb_api::TunnelVerifier`] verifier.
 [@@ FStar.Tactics.Typeclasses.tcinstance]
-let impl_4: t_VerifierSanitizer t_TunnelSecurityRequirements
-  Sandwich_api_proto.Verifiers.t_TunnelVerifier =
+let impl_4: t_VerifierSanitizer #t_TunnelSecurityRequirements
+  #Sandwich_api_proto.Verifiers.t_TunnelVerifier =
   {
     f_run_sanitizer_checks_pre
     =
