proofs/fstar/extraction/Sandwich.Tunnel.Tls.Support.fst
@@ -41,277 +41,6 @@ let tls_options_get_min_max_tls_version (tls_options: Sandwich_api_proto.Tls.t_T
     <:
     (Sandwich.Tunnel.Tls.t_TlsVersion & Sandwich.Tunnel.Tls.t_TlsVersion)
 
-let build_ciphersuites_list
-      (#v_S #impl_995885649_: Type0)
-      (#[FStar.Tactics.Typeclasses.tcresolve ()] i2: Core.Convert.t_AsRef v_S string)
-      (#[FStar.Tactics.Typeclasses.tcresolve ()]
-          i3:
-          Core.Iter.Traits.Collect.t_IntoIterator impl_995885649_)
-      (ciphers: impl_995885649_)
-      (invalid_chars: string)
-     =
-  let output:Alloc.String.t_String = Alloc.String.impl__String__new () in
-  let output:Alloc.String.t_String =
-    Core.Iter.Traits.Iterator.f_fold (Core.Iter.Traits.Collect.f_into_iter #i3.f_IntoIter
-          (Core.Iter.Traits.Collect.f_into_iter #impl_995885649_ ciphers <: i3.f_IntoIter)
-        <:
-        i3.f_IntoIter)
-      output
-      (fun output c ->
-          let output:Alloc.String.t_String = output in
-          let c:v_S = c in
-          let! _:Prims.unit =
-            if
-              Sandwich.Support.contains_any_of (Core.Convert.f_as_ref #v_S #string c <: string)
-                invalid_chars
-            then
-              let! hoist5:Rust_primitives.Hax.t_Never =
-                Core.Ops.Control_flow.ControlFlow_Break
-                (Core.Result.Result_Err
-                  (Core.Convert.f_into #Sandwich_proto.Errors.t_TLSConfigurationError
-                      #Sandwich.Error.t_Error
-                      (Sandwich_proto.Errors.TLSConfigurationError_TLSCONFIGURATIONERROR_UNSUPPORTED_CONTROL_CHARACTERS
-                        <:
-                        Sandwich_proto.Errors.t_TLSConfigurationError))
-                  <:
-                  Core.Result.t_Result Alloc.String.t_String Sandwich.Error.t_Error)
-                <:
-                Core.Ops.Control_flow.t_ControlFlow
-                  (Core.Result.t_Result Alloc.String.t_String Sandwich.Error.t_Error)
-                  Rust_primitives.Hax.t_Never
-              in
-              Core.Ops.Control_flow.ControlFlow_Continue (Rust_primitives.Hax.never_to_any hoist5)
-              <:
-              Core.Ops.Control_flow.t_ControlFlow
-                (Core.Result.t_Result Alloc.String.t_String Sandwich.Error.t_Error) Prims.unit
-            else
-              Core.Ops.Control_flow.ControlFlow_Continue ()
-              <:
-              Core.Ops.Control_flow.t_ControlFlow
-                (Core.Result.t_Result Alloc.String.t_String Sandwich.Error.t_Error) Prims.unit
-          in
-          Core.Ops.Control_flow.ControlFlow_Continue
-          (let output:Alloc.String.t_String =
-              Alloc.String.impl__String__push_str output
-                (Core.Convert.f_as_ref #v_S #string c <: string)
-            in
-            let output:Alloc.String.t_String = Alloc.String.impl__String__push output ':' in
-            output)
-          <:
-          Core.Ops.Control_flow.t_ControlFlow
-            (Core.Result.t_Result Alloc.String.t_String Sandwich.Error.t_Error)
-            Alloc.String.t_String)
-  in
-  let tmp0, out:(Alloc.String.t_String & Core.Option.t_Option char) =
-    Alloc.String.impl__String__pop output
-  in
-  let output:Alloc.String.t_String = tmp0 in
-  let _:Core.Option.t_Option char = out in
-  Core.Result.Result_Ok output <: Core.Result.t_Result Alloc.String.t_String Sandwich.Error.t_Error
-
-let configuration_get_mode_and_options
-      (configuration: Sandwich_api_proto.Configuration.t_Configuration)
-     =
-  Core.Option.impl__ok_or #(Sandwich.Tunnel.Context.t_Mode & Sandwich_api_proto.Tls.t_TLSOptions)
-    #Sandwich.Error.t_Error
-    (Core.Option.impl__and_then #Sandwich_api_proto.Configuration.Configuration.t_Opts
-        #(Sandwich.Tunnel.Context.t_Mode & Sandwich_api_proto.Tls.t_TLSOptions)
-        (Core.Option.impl__as_ref #Sandwich_api_proto.Configuration.Configuration.t_Opts
-            configuration.Sandwich_api_proto.Configuration.f_opts
-          <:
-          Core.Option.t_Option Sandwich_api_proto.Configuration.Configuration.t_Opts)
-        (fun opts ->
-            let opts:Sandwich_api_proto.Configuration.Configuration.t_Opts = opts in
-            match opts with
-            | Sandwich_api_proto.Configuration.Configuration.Opts_Client opt ->
-              Core.Option.impl__map #Sandwich_api_proto.Tls.t_TLSOptions
-                #(Sandwich.Tunnel.Context.t_Mode & Sandwich_api_proto.Tls.t_TLSOptions)
-                (Core.Option.impl__and_then #Sandwich_api_proto.Tls.t_TLSClientOptions
-                    #Sandwich_api_proto.Tls.t_TLSOptions
-                    (Core.Option.impl__and_then #Sandwich_api_proto.Configuration.Client_options.t_Opts
-                        #Sandwich_api_proto.Tls.t_TLSClientOptions
-                        (Core.Option.impl__as_ref #Sandwich_api_proto.Configuration.Client_options.t_Opts
-                            opt.Sandwich_api_proto.Configuration.f_opts
-                          <:
-                          Core.Option.t_Option
-                          Sandwich_api_proto.Configuration.Client_options.t_Opts)
-                        (fun proto ->
-                            let proto:Sandwich_api_proto.Configuration.Client_options.t_Opts =
-                              proto
-                            in
-                            match proto with
-                            | Sandwich_api_proto.Configuration.Client_options.Opts_Tls tls ->
-                              Core.Option.Option_Some tls
-                              <:
-                              Core.Option.t_Option Sandwich_api_proto.Tls.t_TLSClientOptions
-                            | _ ->
-                              Core.Option.Option_None
-                              <:
-                              Core.Option.t_Option Sandwich_api_proto.Tls.t_TLSClientOptions)
-                      <:
-                      Core.Option.t_Option Sandwich_api_proto.Tls.t_TLSClientOptions)
-                    (fun opts ->
-                        let opts:Sandwich_api_proto.Tls.t_TLSClientOptions = opts in
-                        Protobuf.Message_field.impl__as_ref #Sandwich_api_proto.Tls.t_TLSOptions
-                          opts.Sandwich_api_proto.Tls.f_common_options
-                        <:
-                        Core.Option.t_Option Sandwich_api_proto.Tls.t_TLSOptions)
-                  <:
-                  Core.Option.t_Option Sandwich_api_proto.Tls.t_TLSOptions)
-                (fun tls ->
-                    let tls:Sandwich_api_proto.Tls.t_TLSOptions = tls in
-                    (Sandwich.Tunnel.Context.Mode_Client <: Sandwich.Tunnel.Context.t_Mode), tls
-                    <:
-                    (Sandwich.Tunnel.Context.t_Mode & Sandwich_api_proto.Tls.t_TLSOptions))
-              <:
-              Core.Option.t_Option
-              (Sandwich.Tunnel.Context.t_Mode & Sandwich_api_proto.Tls.t_TLSOptions)
-            | Sandwich_api_proto.Configuration.Configuration.Opts_Server opt ->
-              Core.Option.impl__map #Sandwich_api_proto.Tls.t_TLSOptions
-                #(Sandwich.Tunnel.Context.t_Mode & Sandwich_api_proto.Tls.t_TLSOptions)
-                (Core.Option.impl__and_then #Sandwich_api_proto.Tls.t_TLSServerOptions
-                    #Sandwich_api_proto.Tls.t_TLSOptions
-                    (Core.Option.impl__and_then #Sandwich_api_proto.Configuration.Server_options.t_Opts
-                        #Sandwich_api_proto.Tls.t_TLSServerOptions
-                        (Core.Option.impl__as_ref #Sandwich_api_proto.Configuration.Server_options.t_Opts
-                            opt.Sandwich_api_proto.Configuration.f_opts
-                          <:
-                          Core.Option.t_Option
-                          Sandwich_api_proto.Configuration.Server_options.t_Opts)
-                        (fun proto ->
-                            let proto:Sandwich_api_proto.Configuration.Server_options.t_Opts =
-                              proto
-                            in
-                            match proto with
-                            | Sandwich_api_proto.Configuration.Server_options.Opts_Tls tls ->
-                              Core.Option.Option_Some tls
-                              <:
-                              Core.Option.t_Option Sandwich_api_proto.Tls.t_TLSServerOptions
-                            | _ ->
-                              Core.Option.Option_None
-                              <:
-                              Core.Option.t_Option Sandwich_api_proto.Tls.t_TLSServerOptions)
-                      <:
-                      Core.Option.t_Option Sandwich_api_proto.Tls.t_TLSServerOptions)
-                    (fun opts ->
-                        let opts:Sandwich_api_proto.Tls.t_TLSServerOptions = opts in
-                        Protobuf.Message_field.impl__as_ref #Sandwich_api_proto.Tls.t_TLSOptions
-                          opts.Sandwich_api_proto.Tls.f_common_options
-                        <:
-                        Core.Option.t_Option Sandwich_api_proto.Tls.t_TLSOptions)
-                  <:
-                  Core.Option.t_Option Sandwich_api_proto.Tls.t_TLSOptions)
-                (fun tls ->
-                    let tls:Sandwich_api_proto.Tls.t_TLSOptions = tls in
-                    (Sandwich.Tunnel.Context.Mode_Server <: Sandwich.Tunnel.Context.t_Mode), tls
-                    <:
-                    (Sandwich.Tunnel.Context.t_Mode & Sandwich_api_proto.Tls.t_TLSOptions))
-              <:
-              Core.Option.t_Option
-              (Sandwich.Tunnel.Context.t_Mode & Sandwich_api_proto.Tls.t_TLSOptions)
-            | _ ->
-              Rust_primitives.Hax.never_to_any (Core.Panicking.panic "internal error: entered unreachable code"
-
-                  <:
-                  Rust_primitives.Hax.t_Never)
-              <:
-              Core.Option.t_Option
-              (Sandwich.Tunnel.Context.t_Mode & Sandwich_api_proto.Tls.t_TLSOptions))
-      <:
-      Core.Option.t_Option (Sandwich.Tunnel.Context.t_Mode & Sandwich_api_proto.Tls.t_TLSOptions))
-    (Core.Convert.f_into #Sandwich_proto.Errors.t_TLSConfigurationError
-        #Sandwich.Error.t_Error
-        (Sandwich_proto.Errors.TLSConfigurationError_TLSCONFIGURATIONERROR_EMPTY
-          <:
-          Sandwich_proto.Errors.t_TLSConfigurationError)
-      <:
-      Sandwich.Error.t_Error)
-
-let tls_options_get_x509_verifier (tls_options: Sandwich_api_proto.Tls.t_TLSOptions) =
-  Core.Result.impl__and_then #Sandwich_api_proto.Tls.Tlsoptions.t_Peer_verifier
-    #Sandwich.Error.t_Error
-    #(Core.Option.t_Option Sandwich_api_proto.Verifiers.t_X509Verifier)
-    (Core.Option.impl__ok_or #Sandwich_api_proto.Tls.Tlsoptions.t_Peer_verifier
-        #Sandwich.Error.t_Error
-        (Core.Option.impl__as_ref #Sandwich_api_proto.Tls.Tlsoptions.t_Peer_verifier
-            tls_options.Sandwich_api_proto.Tls.f_peer_verifier
-          <:
-          Core.Option.t_Option Sandwich_api_proto.Tls.Tlsoptions.t_Peer_verifier)
-        (Core.Convert.f_into #(Sandwich_proto.Errors.t_TLSConfigurationError & string)
-            #Sandwich.Error.t_Error
-            ((Sandwich_proto.Errors.TLSConfigurationError_TLSCONFIGURATIONERROR_EMPTY
-                <:
-                Sandwich_proto.Errors.t_TLSConfigurationError),
-              "no verifier specified"
-              <:
-              (Sandwich_proto.Errors.t_TLSConfigurationError & string))
-          <:
-          Sandwich.Error.t_Error)
-      <:
-      Core.Result.t_Result Sandwich_api_proto.Tls.Tlsoptions.t_Peer_verifier Sandwich.Error.t_Error)
-    (fun v ->
-        let v:Sandwich_api_proto.Tls.Tlsoptions.t_Peer_verifier = v in
-        match v with
-        | Sandwich_api_proto.Tls.Tlsoptions.Peer_verifier_X509Verifier x509 ->
-          Core.Result.Result_Ok
-          (Core.Option.Option_Some x509
-            <:
-            Core.Option.t_Option Sandwich_api_proto.Verifiers.t_X509Verifier)
-          <:
-          Core.Result.t_Result (Core.Option.t_Option Sandwich_api_proto.Verifiers.t_X509Verifier)
-            Sandwich.Error.t_Error
-        | Sandwich_api_proto.Tls.Tlsoptions.Peer_verifier_EmptyVerifier _ ->
-          Core.Result.Result_Ok
-          (Core.Option.Option_None
-            <:
-            Core.Option.t_Option Sandwich_api_proto.Verifiers.t_X509Verifier)
-          <:
-          Core.Result.t_Result (Core.Option.t_Option Sandwich_api_proto.Verifiers.t_X509Verifier)
-            Sandwich.Error.t_Error
-        | _ ->
-          Rust_primitives.Hax.never_to_any (Core.Panicking.panic "internal error: entered unreachable code"
-
-              <:
-              Rust_primitives.Hax.t_Never)
-          <:
-          Core.Result.t_Result (Core.Option.t_Option Sandwich_api_proto.Verifiers.t_X509Verifier)
-            Sandwich.Error.t_Error)
-
-let x509_verifier_verify_emptiness
-      (x509_verifier: Core.Option.t_Option Sandwich_api_proto.Verifiers.t_X509Verifier)
-     =
-  match x509_verifier with
-  | Core.Option.Option_Some x509 ->
-    if
-      Alloc.Vec.impl_1__is_empty #Sandwich_api_proto.Certificate.t_Certificate
-        #Alloc.Alloc.t_Global
-        x509.Sandwich_api_proto.Verifiers.f_trusted_cas &&
-      ~.x509.Sandwich_api_proto.Verifiers.f_load_cas_from_default_verify_path
-    then
-      Core.Result.Result_Err
-      (Core.Convert.f_into #(Sandwich_proto.Errors.t_TLSConfigurationError & string)
-          #Sandwich.Error.t_Error
-          ((Sandwich_proto.Errors.TLSConfigurationError_TLSCONFIGURATIONERROR_EMPTY
-              <:
-              Sandwich_proto.Errors.t_TLSConfigurationError),
-            "X.509 verifier empty"
-            <:
-            (Sandwich_proto.Errors.t_TLSConfigurationError & string)))
-      <:
-      Core.Result.t_Result (Core.Option.t_Option Sandwich_api_proto.Verifiers.t_X509Verifier)
-        Sandwich.Error.t_Error
-    else
-      Core.Result.Result_Ok x509_verifier
-      <:
-      Core.Result.t_Result (Core.Option.t_Option Sandwich_api_proto.Verifiers.t_X509Verifier)
-        Sandwich.Error.t_Error
-  | _ ->
-    Core.Result.Result_Ok
-    (Core.Option.Option_None <: Core.Option.t_Option Sandwich_api_proto.Verifiers.t_X509Verifier)
-    <:
-    Core.Result.t_Result (Core.Option.t_Option Sandwich_api_proto.Verifiers.t_X509Verifier)
-      Sandwich.Error.t_Error
-
 let configuration_read_certificate (cert: Sandwich_api_proto.Certificate.t_Certificate) =
   Core.Result.impl__and_then #Sandwich_api_proto.Certificate.Certificate.t_Source
     #Sandwich.Error.t_Error
@@ -529,3 +258,274 @@ let configuration_read_private_key (private_key: Sandwich_api_proto.Private_key.
           Core.Result.t_Result
             (Sandwich_api_proto.Encoding_format.t_ASN1EncodingFormat &
               Sandwich.Support.Data_source.t_DataSource) Sandwich.Error.t_Error)
+
+let configuration_get_mode_and_options
+      (configuration: Sandwich_api_proto.Configuration.t_Configuration)
+     =
+  Core.Option.impl__ok_or #(Sandwich.Tunnel.Context.t_Mode & Sandwich_api_proto.Tls.t_TLSOptions)
+    #Sandwich.Error.t_Error
+    (Core.Option.impl__and_then #Sandwich_api_proto.Configuration.Configuration.t_Opts
+        #(Sandwich.Tunnel.Context.t_Mode & Sandwich_api_proto.Tls.t_TLSOptions)
+        (Core.Option.impl__as_ref #Sandwich_api_proto.Configuration.Configuration.t_Opts
+            configuration.Sandwich_api_proto.Configuration.f_opts
+          <:
+          Core.Option.t_Option Sandwich_api_proto.Configuration.Configuration.t_Opts)
+        (fun opts ->
+            let opts:Sandwich_api_proto.Configuration.Configuration.t_Opts = opts in
+            match opts with
+            | Sandwich_api_proto.Configuration.Configuration.Opts_Client opt ->
+              Core.Option.impl__map #Sandwich_api_proto.Tls.t_TLSOptions
+                #(Sandwich.Tunnel.Context.t_Mode & Sandwich_api_proto.Tls.t_TLSOptions)
+                (Core.Option.impl__and_then #Sandwich_api_proto.Tls.t_TLSClientOptions
+                    #Sandwich_api_proto.Tls.t_TLSOptions
+                    (Core.Option.impl__and_then #Sandwich_api_proto.Configuration.Client_options.t_Opts
+                        #Sandwich_api_proto.Tls.t_TLSClientOptions
+                        (Core.Option.impl__as_ref #Sandwich_api_proto.Configuration.Client_options.t_Opts
+                            opt.Sandwich_api_proto.Configuration.f_opts
+                          <:
+                          Core.Option.t_Option
+                          Sandwich_api_proto.Configuration.Client_options.t_Opts)
+                        (fun proto ->
+                            let proto:Sandwich_api_proto.Configuration.Client_options.t_Opts =
+                              proto
+                            in
+                            match proto with
+                            | Sandwich_api_proto.Configuration.Client_options.Opts_Tls tls ->
+                              Core.Option.Option_Some tls
+                              <:
+                              Core.Option.t_Option Sandwich_api_proto.Tls.t_TLSClientOptions
+                            | _ ->
+                              Core.Option.Option_None
+                              <:
+                              Core.Option.t_Option Sandwich_api_proto.Tls.t_TLSClientOptions)
+                      <:
+                      Core.Option.t_Option Sandwich_api_proto.Tls.t_TLSClientOptions)
+                    (fun opts ->
+                        let opts:Sandwich_api_proto.Tls.t_TLSClientOptions = opts in
+                        Protobuf.Message_field.impl__as_ref #Sandwich_api_proto.Tls.t_TLSOptions
+                          opts.Sandwich_api_proto.Tls.f_common_options
+                        <:
+                        Core.Option.t_Option Sandwich_api_proto.Tls.t_TLSOptions)
+                  <:
+                  Core.Option.t_Option Sandwich_api_proto.Tls.t_TLSOptions)
+                (fun tls ->
+                    let tls:Sandwich_api_proto.Tls.t_TLSOptions = tls in
+                    (Sandwich.Tunnel.Context.Mode_Client <: Sandwich.Tunnel.Context.t_Mode), tls
+                    <:
+                    (Sandwich.Tunnel.Context.t_Mode & Sandwich_api_proto.Tls.t_TLSOptions))
+              <:
+              Core.Option.t_Option
+              (Sandwich.Tunnel.Context.t_Mode & Sandwich_api_proto.Tls.t_TLSOptions)
+            | Sandwich_api_proto.Configuration.Configuration.Opts_Server opt ->
+              Core.Option.impl__map #Sandwich_api_proto.Tls.t_TLSOptions
+                #(Sandwich.Tunnel.Context.t_Mode & Sandwich_api_proto.Tls.t_TLSOptions)
+                (Core.Option.impl__and_then #Sandwich_api_proto.Tls.t_TLSServerOptions
+                    #Sandwich_api_proto.Tls.t_TLSOptions
+                    (Core.Option.impl__and_then #Sandwich_api_proto.Configuration.Server_options.t_Opts
+                        #Sandwich_api_proto.Tls.t_TLSServerOptions
+                        (Core.Option.impl__as_ref #Sandwich_api_proto.Configuration.Server_options.t_Opts
+                            opt.Sandwich_api_proto.Configuration.f_opts
+                          <:
+                          Core.Option.t_Option
+                          Sandwich_api_proto.Configuration.Server_options.t_Opts)
+                        (fun proto ->
+                            let proto:Sandwich_api_proto.Configuration.Server_options.t_Opts =
+                              proto
+                            in
+                            match proto with
+                            | Sandwich_api_proto.Configuration.Server_options.Opts_Tls tls ->
+                              Core.Option.Option_Some tls
+                              <:
+                              Core.Option.t_Option Sandwich_api_proto.Tls.t_TLSServerOptions
+                            | _ ->
+                              Core.Option.Option_None
+                              <:
+                              Core.Option.t_Option Sandwich_api_proto.Tls.t_TLSServerOptions)
+                      <:
+                      Core.Option.t_Option Sandwich_api_proto.Tls.t_TLSServerOptions)
+                    (fun opts ->
+                        let opts:Sandwich_api_proto.Tls.t_TLSServerOptions = opts in
+                        Protobuf.Message_field.impl__as_ref #Sandwich_api_proto.Tls.t_TLSOptions
+                          opts.Sandwich_api_proto.Tls.f_common_options
+                        <:
+                        Core.Option.t_Option Sandwich_api_proto.Tls.t_TLSOptions)
+                  <:
+                  Core.Option.t_Option Sandwich_api_proto.Tls.t_TLSOptions)
+                (fun tls ->
+                    let tls:Sandwich_api_proto.Tls.t_TLSOptions = tls in
+                    (Sandwich.Tunnel.Context.Mode_Server <: Sandwich.Tunnel.Context.t_Mode), tls
+                    <:
+                    (Sandwich.Tunnel.Context.t_Mode & Sandwich_api_proto.Tls.t_TLSOptions))
+              <:
+              Core.Option.t_Option
+              (Sandwich.Tunnel.Context.t_Mode & Sandwich_api_proto.Tls.t_TLSOptions)
+            | _ ->
+              Rust_primitives.Hax.never_to_any (Core.Panicking.panic "internal error: entered unreachable code"
+
+                  <:
+                  Rust_primitives.Hax.t_Never)
+              <:
+              Core.Option.t_Option
+              (Sandwich.Tunnel.Context.t_Mode & Sandwich_api_proto.Tls.t_TLSOptions))
+      <:
+      Core.Option.t_Option (Sandwich.Tunnel.Context.t_Mode & Sandwich_api_proto.Tls.t_TLSOptions))
+    (Core.Convert.f_into #Sandwich_proto.Errors.t_TLSConfigurationError
+        #Sandwich.Error.t_Error
+        (Sandwich_proto.Errors.TLSConfigurationError_TLSCONFIGURATIONERROR_EMPTY
+          <:
+          Sandwich_proto.Errors.t_TLSConfigurationError)
+      <:
+      Sandwich.Error.t_Error)
+
+let tls_options_get_x509_verifier (tls_options: Sandwich_api_proto.Tls.t_TLSOptions) =
+  Core.Result.impl__and_then #Sandwich_api_proto.Tls.Tlsoptions.t_Peer_verifier
+    #Sandwich.Error.t_Error
+    #(Core.Option.t_Option Sandwich_api_proto.Verifiers.t_X509Verifier)
+    (Core.Option.impl__ok_or #Sandwich_api_proto.Tls.Tlsoptions.t_Peer_verifier
+        #Sandwich.Error.t_Error
+        (Core.Option.impl__as_ref #Sandwich_api_proto.Tls.Tlsoptions.t_Peer_verifier
+            tls_options.Sandwich_api_proto.Tls.f_peer_verifier
+          <:
+          Core.Option.t_Option Sandwich_api_proto.Tls.Tlsoptions.t_Peer_verifier)
+        (Core.Convert.f_into #(Sandwich_proto.Errors.t_TLSConfigurationError & string)
+            #Sandwich.Error.t_Error
+            ((Sandwich_proto.Errors.TLSConfigurationError_TLSCONFIGURATIONERROR_EMPTY
+                <:
+                Sandwich_proto.Errors.t_TLSConfigurationError),
+              "no verifier specified"
+              <:
+              (Sandwich_proto.Errors.t_TLSConfigurationError & string))
+          <:
+          Sandwich.Error.t_Error)
+      <:
+      Core.Result.t_Result Sandwich_api_proto.Tls.Tlsoptions.t_Peer_verifier Sandwich.Error.t_Error)
+    (fun v ->
+        let v:Sandwich_api_proto.Tls.Tlsoptions.t_Peer_verifier = v in
+        match v with
+        | Sandwich_api_proto.Tls.Tlsoptions.Peer_verifier_X509Verifier x509 ->
+          Core.Result.Result_Ok
+          (Core.Option.Option_Some x509
+            <:
+            Core.Option.t_Option Sandwich_api_proto.Verifiers.t_X509Verifier)
+          <:
+          Core.Result.t_Result (Core.Option.t_Option Sandwich_api_proto.Verifiers.t_X509Verifier)
+            Sandwich.Error.t_Error
+        | Sandwich_api_proto.Tls.Tlsoptions.Peer_verifier_EmptyVerifier _ ->
+          Core.Result.Result_Ok
+          (Core.Option.Option_None
+            <:
+            Core.Option.t_Option Sandwich_api_proto.Verifiers.t_X509Verifier)
+          <:
+          Core.Result.t_Result (Core.Option.t_Option Sandwich_api_proto.Verifiers.t_X509Verifier)
+            Sandwich.Error.t_Error
+        | _ ->
+          Rust_primitives.Hax.never_to_any (Core.Panicking.panic "internal error: entered unreachable code"
+
+              <:
+              Rust_primitives.Hax.t_Never)
+          <:
+          Core.Result.t_Result (Core.Option.t_Option Sandwich_api_proto.Verifiers.t_X509Verifier)
+            Sandwich.Error.t_Error)
+
+let x509_verifier_verify_emptiness
+      (x509_verifier: Core.Option.t_Option Sandwich_api_proto.Verifiers.t_X509Verifier)
+     =
+  match x509_verifier with
+  | Core.Option.Option_Some x509 ->
+    if
+      Alloc.Vec.impl_1__is_empty #Sandwich_api_proto.Certificate.t_Certificate
+        #Alloc.Alloc.t_Global
+        x509.Sandwich_api_proto.Verifiers.f_trusted_cas &&
+      ~.x509.Sandwich_api_proto.Verifiers.f_load_cas_from_default_verify_path
+    then
+      Core.Result.Result_Err
+      (Core.Convert.f_into #(Sandwich_proto.Errors.t_TLSConfigurationError & string)
+          #Sandwich.Error.t_Error
+          ((Sandwich_proto.Errors.TLSConfigurationError_TLSCONFIGURATIONERROR_EMPTY
+              <:
+              Sandwich_proto.Errors.t_TLSConfigurationError),
+            "X.509 verifier empty"
+            <:
+            (Sandwich_proto.Errors.t_TLSConfigurationError & string)))
+      <:
+      Core.Result.t_Result (Core.Option.t_Option Sandwich_api_proto.Verifiers.t_X509Verifier)
+        Sandwich.Error.t_Error
+    else
+      Core.Result.Result_Ok x509_verifier
+      <:
+      Core.Result.t_Result (Core.Option.t_Option Sandwich_api_proto.Verifiers.t_X509Verifier)
+        Sandwich.Error.t_Error
+  | _ ->
+    Core.Result.Result_Ok
+    (Core.Option.Option_None <: Core.Option.t_Option Sandwich_api_proto.Verifiers.t_X509Verifier)
+    <:
+    Core.Result.t_Result (Core.Option.t_Option Sandwich_api_proto.Verifiers.t_X509Verifier)
+      Sandwich.Error.t_Error
+
+let build_ciphersuites_list
+      (#v_S #impl_995885649_: Type0)
+      (#[FStar.Tactics.Typeclasses.tcresolve ()] i2: Core.Convert.t_AsRef v_S string)
+      (#[FStar.Tactics.Typeclasses.tcresolve ()]
+          i3:
+          Core.Iter.Traits.Collect.t_IntoIterator impl_995885649_)
+      (ciphers: impl_995885649_)
+      (invalid_chars: string)
+     =
+  let output:Alloc.String.t_String = Alloc.String.impl__String__new () in
+  let output:Alloc.String.t_String =
+    Core.Iter.Traits.Iterator.f_fold (Core.Iter.Traits.Collect.f_into_iter #i3.f_IntoIter
+          (Core.Iter.Traits.Collect.f_into_iter #impl_995885649_ ciphers <: i3.f_IntoIter)
+        <:
+        i3.f_IntoIter)
+      output
+      (fun output c ->
+          let output:Alloc.String.t_String = output in
+          let c:v_S = c in
+          let! _:Prims.unit =
+            if
+              Sandwich.Support.contains_any_of (Core.Convert.f_as_ref #v_S #string c <: string)
+                invalid_chars
+            then
+              let! hoist2:Rust_primitives.Hax.t_Never =
+                Core.Ops.Control_flow.ControlFlow_Break
+                (Core.Result.Result_Err
+                  (Core.Convert.f_into #Sandwich_proto.Errors.t_TLSConfigurationError
+                      #Sandwich.Error.t_Error
+                      (Sandwich_proto.Errors.TLSConfigurationError_TLSCONFIGURATIONERROR_UNSUPPORTED_CONTROL_CHARACTERS
+                        <:
+                        Sandwich_proto.Errors.t_TLSConfigurationError))
+                  <:
+                  Core.Result.t_Result Alloc.String.t_String Sandwich.Error.t_Error)
+                <:
+                Core.Ops.Control_flow.t_ControlFlow
+                  (Core.Result.t_Result Alloc.String.t_String Sandwich.Error.t_Error)
+                  Rust_primitives.Hax.t_Never
+              in
+              Core.Ops.Control_flow.ControlFlow_Continue (Rust_primitives.Hax.never_to_any hoist2)
+              <:
+              Core.Ops.Control_flow.t_ControlFlow
+                (Core.Result.t_Result Alloc.String.t_String Sandwich.Error.t_Error) Prims.unit
+            else
+              Core.Ops.Control_flow.ControlFlow_Continue ()
+              <:
+              Core.Ops.Control_flow.t_ControlFlow
+                (Core.Result.t_Result Alloc.String.t_String Sandwich.Error.t_Error) Prims.unit
+          in
+          Core.Ops.Control_flow.ControlFlow_Continue
+          (let output:Alloc.String.t_String =
+              Alloc.String.impl__String__push_str output
+                (Core.Convert.f_as_ref #v_S #string c <: string)
+            in
+            let output:Alloc.String.t_String = Alloc.String.impl__String__push output ':' in
+            output)
+          <:
+          Core.Ops.Control_flow.t_ControlFlow
+            (Core.Result.t_Result Alloc.String.t_String Sandwich.Error.t_Error)
+            Alloc.String.t_String)
+  in
+  let tmp0, out:(Alloc.String.t_String & Core.Option.t_Option char) =
+    Alloc.String.impl__String__pop output
+  in
+  let output:Alloc.String.t_String = tmp0 in
+  let _:Core.Option.t_Option char = out in
+  Core.Result.Result_Ok output <: Core.Result.t_Result Alloc.String.t_String Sandwich.Error.t_Error
