rust_vendor/openssl3/proofs/fstar/extraction/Openssl3.fsti
@@ -1,0 +1,6 @@
+module Openssl3
+#set-options "--fuel 0 --ifuel 1 --z3rlimit 15"
+open Core
+open FStar.Mul
+
+let v_X509_V_ERR_CERT_HAS_EXPIRED: u32 = Rust_primitives.Hax.dropped_body
