rust_vendor/sandwich-api-proto/proofs/fstar/extraction/Sandwich_api_proto.Certificate.fsti
@@ -1,0 +1,9 @@
+module Sandwich_api_proto.Certificate
+#set-options "--fuel 0 --ifuel 1 --z3rlimit 15"
+open Core
+open FStar.Mul
+
+type t_Certificate = {
+  f_source:Core.Option.t_Option Sandwich_api_proto.Certificate.Certificate.t_Source;
+  f_special_fields:Protobuf.Special.t_SpecialFields
+}
