rust_vendor/sandwich-api-proto/proofs/fstar/extraction/Sandwich_api_proto.Compliance.fsti
@@ -1,0 +1,89 @@
+module Sandwich_api_proto.Compliance
+#set-options "--fuel 0 --ifuel 1 --z3rlimit 15"
+open Core
+open FStar.Mul
+
+let _ =
+  (* This module has implicit dependencies, here we make them explicit. *)
+  (* The implicit dependencies arise from typeclasses instances. *)
+  let open Protobuf.Enums in
+  let open Protobuf.Message in
+  let open Protobuf.Reflect.Runtime_types in
+  let open Protobuf.Reflect.Value in
+  ()
+
+type t_ClassicalAlgoChoice =
+  | ClassicalAlgoChoice_CLASSICAL_ALGORITHMS_ALLOW : t_ClassicalAlgoChoice
+  | ClassicalAlgoChoice_CLASSICAL_ALGORITHMS_FORBID : t_ClassicalAlgoChoice
+
+[@@ FStar.Tactics.Typeclasses.tcinstance]
+val impl_8:Core.Default.t_Default #t_ClassicalAlgoChoice
+
+[@@ FStar.Tactics.Typeclasses.tcinstance]
+val impl_6:Protobuf.Enums.t_Enum #t_ClassicalAlgoChoice
+
+[@@ FStar.Tactics.Typeclasses.tcinstance]
+val impl_7:Protobuf.Enum_full.t_EnumFull #t_ClassicalAlgoChoice
+
+type t_HybridAlgoChoice =
+  | HybridAlgoChoice_HYBRID_ALGORITHMS_ALLOW : t_HybridAlgoChoice
+  | HybridAlgoChoice_HYBRID_ALGORITHMS_FORBID : t_HybridAlgoChoice
+
+[@@ FStar.Tactics.Typeclasses.tcinstance]
+val impl_16:Core.Default.t_Default #t_HybridAlgoChoice
+
+[@@ FStar.Tactics.Typeclasses.tcinstance]
+val impl_14:Protobuf.Enums.t_Enum #t_HybridAlgoChoice
+
+[@@ FStar.Tactics.Typeclasses.tcinstance]
+val impl_15:Protobuf.Enum_full.t_EnumFull #t_HybridAlgoChoice
+
+type t_NISTSecurityStrengthBits =
+  | NISTSecurityStrengthBits_BIT_STRENGTH_AT_LEAST_128_ : t_NISTSecurityStrengthBits
+  | NISTSecurityStrengthBits_BIT_STRENGTH_AT_LEAST_192_ : t_NISTSecurityStrengthBits
+  | NISTSecurityStrengthBits_BIT_STRENGTH_AT_LEAST_256_ : t_NISTSecurityStrengthBits
+
+[@@ FStar.Tactics.Typeclasses.tcinstance]
+val impl_20:Core.Default.t_Default #t_NISTSecurityStrengthBits
+
+[@@ FStar.Tactics.Typeclasses.tcinstance]
+val impl_18:Protobuf.Enums.t_Enum #t_NISTSecurityStrengthBits
+
+[@@ FStar.Tactics.Typeclasses.tcinstance]
+val impl_19:Protobuf.Enum_full.t_EnumFull #t_NISTSecurityStrengthBits
+
+type t_QuantumSafeAlgoChoice =
+  | QuantumSafeAlgoChoice_QUANTUM_SAFE_ALGORITHMS_ALLOW : t_QuantumSafeAlgoChoice
+  | QuantumSafeAlgoChoice_QUANTUM_SAFE_ALGORITHMS_FORBID : t_QuantumSafeAlgoChoice
+
+[@@ FStar.Tactics.Typeclasses.tcinstance]
+val impl_12:Core.Default.t_Default #t_QuantumSafeAlgoChoice
+
+[@@ FStar.Tactics.Typeclasses.tcinstance]
+val impl_10:Protobuf.Enums.t_Enum #t_QuantumSafeAlgoChoice
+
+[@@ FStar.Tactics.Typeclasses.tcinstance]
+val impl_11:Protobuf.Enum_full.t_EnumFull #t_QuantumSafeAlgoChoice
+
+type t_Compliance = {
+  f_hybrid_choice:Protobuf.Enum_or_unknown.t_EnumOrUnknown t_HybridAlgoChoice;
+  f_quantum_safe_choice:Protobuf.Enum_or_unknown.t_EnumOrUnknown t_QuantumSafeAlgoChoice;
+  f_classical_choice:Protobuf.Enum_or_unknown.t_EnumOrUnknown t_ClassicalAlgoChoice;
+  f_bit_strength_choice:Protobuf.Enum_or_unknown.t_EnumOrUnknown t_NISTSecurityStrengthBits;
+  f_special_fields:Protobuf.Special.t_SpecialFields
+}
+
+[@@ FStar.Tactics.Typeclasses.tcinstance]
+val impl:Core.Default.t_Default #t_Compliance
+
+[@@ FStar.Tactics.Typeclasses.tcinstance]
+val impl_2:Protobuf.Message.t_Message #t_Compliance
+
+[@@ FStar.Tactics.Typeclasses.tcinstance]
+val impl_4:Core.Fmt.t_Display #t_Compliance
+
+[@@ FStar.Tactics.Typeclasses.tcinstance]
+val impl_3:Protobuf.Message_full.t_MessageFull #t_Compliance
+
+[@@ FStar.Tactics.Typeclasses.tcinstance]
+val impl_5:Protobuf.Reflect.Value.t_ProtobufValue #t_Compliance
