rust_vendor/sandwich-api-proto/proofs/fstar/extraction/Sandwich_api_proto.Configuration.Client_options.fsti
@@ -1,0 +1,6 @@
+module Sandwich_api_proto.Configuration.Client_options
+#set-options "--fuel 0 --ifuel 1 --z3rlimit 15"
+open Core
+open FStar.Mul
+
+type t_Opts = | Opts_Tls : Sandwich_api_proto.Tls.t_TLSClientOptions -> t_Opts
