rust_vendor/sandwich-api-proto/proofs/fstar/extraction/Sandwich_api_proto.Configuration.Configuration.fsti
@@ -1,0 +1,8 @@
+module Sandwich_api_proto.Configuration.Configuration
+#set-options "--fuel 0 --ifuel 1 --z3rlimit 15"
+open Core
+open FStar.Mul
+
+type t_Opts =
+  | Opts_Client : Sandwich_api_proto.Configuration.t_ClientOptions -> t_Opts
+  | Opts_Server : Sandwich_api_proto.Configuration.t_ServerOptions -> t_Opts
