rust_vendor/sandwich-api-proto/proofs/fstar/extraction/Sandwich_api_proto.Configuration.fsti
@@ -1,0 +1,20 @@
+module Sandwich_api_proto.Configuration
+#set-options "--fuel 0 --ifuel 1 --z3rlimit 15"
+open Core
+open FStar.Mul
+
+type t_ClientOptions = {
+  f_opts:Core.Option.t_Option Sandwich_api_proto.Configuration.Client_options.t_Opts;
+  f_special_fields:Protobuf.Special.t_SpecialFields
+}
+
+type t_ServerOptions = {
+  f_opts:Core.Option.t_Option Sandwich_api_proto.Configuration.Server_options.t_Opts;
+  f_special_fields:Protobuf.Special.t_SpecialFields
+}
+
+type t_Configuration = {
+  f_impl___:Protobuf.Enum_or_unknown.t_EnumOrUnknown t_Implementation;
+  f_opts:Core.Option.t_Option Sandwich_api_proto.Configuration.Configuration.t_Opts;
+  f_special_fields:Protobuf.Special.t_SpecialFields
+}
