rust_vendor/sandwich-api-proto/proofs/fstar/extraction/Sandwich_api_proto.Data_source.fsti
@@ -1,0 +1,16 @@
+module Sandwich_api_proto.Data_source
+#set-options "--fuel 0 --ifuel 1 --z3rlimit 15"
+open Core
+open FStar.Mul
+
+type t_DataSource = {
+  f_specifier:Core.Option.t_Option Sandwich_api_proto.Data_source.Data_source.t_Specifier;
+  f_special_fields:Protobuf.Special.t_SpecialFields
+}
+
+type t_ASN1DataSource = {
+  f_data:Protobuf.Message_field.t_MessageField t_DataSource;
+  f_format:Protobuf.Enum_or_unknown.t_EnumOrUnknown
+  Sandwich_api_proto.Encoding_format.t_ASN1EncodingFormat;
+  f_special_fields:Protobuf.Special.t_SpecialFields
+}
