rust_vendor/sandwich-api-proto/proofs/fstar/extraction/Sandwich_api_proto.Encoding_format.fsti
@@ -1,0 +1,8 @@
+module Sandwich_api_proto.Encoding_format
+#set-options "--fuel 0 --ifuel 1 --z3rlimit 15"
+open Core
+open FStar.Mul
+
+type t_ASN1EncodingFormat =
+  | ASN1EncodingFormat_ENCODING_FORMAT_PEM : t_ASN1EncodingFormat
+  | ASN1EncodingFormat_ENCODING_FORMAT_DER : t_ASN1EncodingFormat
