rust_vendor/sandwich-api-proto/proofs/fstar/extraction/Sandwich_api_proto.Private_key.Private_key.fsti
@@ -1,0 +1,6 @@
+module Sandwich_api_proto.Private_key.Private_key
+#set-options "--fuel 0 --ifuel 1 --z3rlimit 15"
+open Core
+open FStar.Mul
+
+type t_Source = | Source_Static : Sandwich_api_proto.Data_source.t_ASN1DataSource -> t_Source
