rust_vendor/sandwich-api-proto/proofs/fstar/extraction/Sandwich_api_proto.Tls.Tlsoptions.fsti
@@ -1,0 +1,8 @@
+module Sandwich_api_proto.Tls.Tlsoptions
+#set-options "--fuel 0 --ifuel 1 --z3rlimit 15"
+open Core
+open FStar.Mul
+
+type t_Peer_verifier =
+  | Peer_verifier_X509Verifier : Sandwich_api_proto.Verifiers.t_X509Verifier -> t_Peer_verifier
+  | Peer_verifier_EmptyVerifier : Sandwich_api_proto.Verifiers.t_EmptyVerifier -> t_Peer_verifier
