rust_vendor/sandwich-api-proto/proofs/fstar/extraction/Sandwich_api_proto.Verifiers.Sanmatcher.fsti
@@ -1,0 +1,21 @@
+module Sandwich_api_proto.Verifiers.Sanmatcher
+#set-options "--fuel 0 --ifuel 1 --z3rlimit 15"
+open Core
+open FStar.Mul
+
+let _ =
+  (* This module has implicit dependencies, here we make them explicit. *)
+  (* The implicit dependencies arise from typeclasses instances. *)
+  let open Protobuf.Oneof in
+  ()
+
+type t_San =
+  | San_Email : Alloc.String.t_String -> t_San
+  | San_Dns : Alloc.String.t_String -> t_San
+  | San_IpAddress : Alloc.String.t_String -> t_San
+
+[@@ FStar.Tactics.Typeclasses.tcinstance]
+val impl:Protobuf.Oneof.t_Oneof #t_San
+
+[@@ FStar.Tactics.Typeclasses.tcinstance]
+val impl_1:Protobuf.Oneof_full.t_OneofFull #t_San
