rust_vendor/sandwich-api-proto/proofs/fstar/extraction/Sandwich_api_proto.Verifiers.Tunnel_verifier.fsti
@@ -1,0 +1,8 @@
+module Sandwich_api_proto.Verifiers.Tunnel_verifier
+#set-options "--fuel 0 --ifuel 1 --z3rlimit 15"
+open Core
+open FStar.Mul
+
+type t_Verifier =
+  | Verifier_SanVerifier : Sandwich_api_proto.Verifiers.t_SANVerifier -> t_Verifier
+  | Verifier_EmptyVerifier : Sandwich_api_proto.Verifiers.t_EmptyVerifier -> t_Verifier
