rust_vendor/sandwich-api-proto/proofs/fstar/extraction/Sandwich_api_proto.Verifiers.fsti
@@ -1,0 +1,29 @@
+module Sandwich_api_proto.Verifiers
+#set-options "--fuel 0 --ifuel 1 --z3rlimit 15"
+open Core
+open FStar.Mul
+
+type t_EmptyVerifier = { f_special_fields:Protobuf.Special.t_SpecialFields }
+
+type t_SANMatcher = {
+  f_san:Core.Option.t_Option Sandwich_api_proto.Verifiers.Sanmatcher.t_San;
+  f_special_fields:Protobuf.Special.t_SpecialFields
+}
+
+type t_SANVerifier = {
+  f_alt_names:Alloc.Vec.t_Vec t_SANMatcher Alloc.Alloc.t_Global;
+  f_special_fields:Protobuf.Special.t_SpecialFields
+}
+
+type t_TunnelVerifier = {
+  f_verifier:Core.Option.t_Option Sandwich_api_proto.Verifiers.Tunnel_verifier.t_Verifier;
+  f_special_fields:Protobuf.Special.t_SpecialFields
+}
+
+type t_X509Verifier = {
+  f_trusted_cas:Alloc.Vec.t_Vec Sandwich_api_proto.Certificate.t_Certificate Alloc.Alloc.t_Global;
+  f_allow_expired_certificate:bool;
+  f_max_verify_depth:u32;
+  f_load_cas_from_default_verify_path:bool;
+  f_special_fields:Protobuf.Special.t_SpecialFields
+}
